+++
title = "Binomial theorem"
author = ["Cash Prokop-Weaver"]
date = 2023-01-19T09:49:00-08:00
lastmod = 2023-09-24T09:56:16-07:00
tags = ["concept", "concept"]
categories = ["concept"]
draft = false
slug = "e3806f4b-94b7-443e-8e7e-278fe8a2781c"
+++

> In elementary algebra, the binomial theorem (or binomial expansion) describes the algebraic expansion of powers of a binomial. According to the theorem, it is possible to expand the polynomial \\((x + y)^n\\) into a sum involving terms of the form \\(ax^by^c\\), where the exponents \\(b\\) and \\(c\\) are nonnegative integers with \\(b + c = n\\), and the coefficient \\(a\\) of each term is a specific positive integer depending on \\(n\\) and \\(b\\). For example, for \\(n = 4\\),
>
> \\((x+y)^{4}=x^{4}+4x^{3}y+6x^{2}y^{2}+4xy^{3}+y^{4}\\)
>
> The coefficient a in the term of \\(ax^by^c\\) is known as the binomial coefficient [[Binomial coefficient]({{< relref "binomial_coefficient.md" >}})] \\(\binom{n}{b}\\) or \\(\tbinom {n}{c}}\\) (the two have the same value).
>
> (<a href="#citeproc_bib_item_1">“Binomial Theorem” 2023</a>)

<!--quoteend-->

> $$
>
> \begin{align}
> (x+y)^{n} &=\sum \_{k=0}^{n}{n \choose k}x^{n-k}y^{k} \\\\
> &=\sum \_{k=0}^{n}{n \choose k}x^{k}y^{n-k}
> \end{align}
>
> $$
>
> (<a href="#citeproc_bib_item_1">“Binomial Theorem” 2023</a>)


## Flashcards {#flashcards}


### Equivalence {#equivalence}

| position | ease | box | interval | due                  |
|----------|------|-----|----------|----------------------|
| 0        | 2.50 | 7   | 304.24   | 2024-06-09T06:28:48Z |
| 1        | 1.30 | 4   | 7.71     | 2023-09-22T08:27:27Z |

{{\\((x+y)^{n}\\)}@0} \\(=\\) {{\\(\sum \_{k=0}^{n}{n \choose k}x^{k}y^{n-k}\\)}{summation}@1}


#### Source {#source}

(<a href="#citeproc_bib_item_1">“Binomial Theorem” 2023</a>)


### Definition {#definition}

| position | ease | box | interval | due                  |
|----------|------|-----|----------|----------------------|
| front    | 1.75 | 8   | 95.42    | 2023-12-14T09:09:15Z |
| back     | 2.20 | 7   | 207.64   | 2024-02-23T15:21:23Z |

[Binomial theorem]({{< relref "binomial_theorem.md" >}})


#### Back {#back}

$$

\begin{align}
(x+y)^{n} &=\sum \_{k=0}^{n}{n \choose k}x^{n-k}y^{k} \\\\
&=\sum \_{k=0}^{n}{n \choose k}x^{k}y^{n-k}
\end{align}

$$


#### Source {#source}

(<a href="#citeproc_bib_item_1">“Binomial Theorem” 2023</a>)


### Describe {#describe}

| position | ease | box | interval | due                  |
|----------|------|-----|----------|----------------------|
| front    | 2.35 | 7   | 203.58   | 2024-01-13T03:59:20Z |

Relationship between the [Binomial theorem]({{< relref "binomial_theorem.md" >}}) and [Binomial coefficient]({{< relref "binomial_coefficient.md" >}})


#### Back {#back}

The [Binomial coefficient]({{< relref "binomial_coefficient.md" >}}) is the coefficient in the [Binomial theorem]({{< relref "binomial_theorem.md" >}})'s summation:

$$

\begin{align}
(x+y)^{n} &=\sum \_{k=0}^{n}{n \choose k}x^{n-k}y^{k} \\\\
&=\sum \_{k=0}^{n}{n \choose k}x^{k}y^{n-k}
\end{align}

$$


#### Source {#source}

(<a href="#citeproc_bib_item_1">“Binomial Theorem” 2023</a>)

## References

<style>.csl-entry{text-indent: -1.5em; margin-left: 1.5em;}</style><div class="csl-bib-body">
  <div class="csl-entry"><a id="citeproc_bib_item_1"></a>“Binomial Theorem.” 2023. In <i>Wikipedia</i>. <a href="https://en.wikipedia.org/w/index.php?title=Binomial_theorem&oldid=1133606899">https://en.wikipedia.org/w/index.php?title=Binomial_theorem&#38;oldid=1133606899</a>.</div>
</div>


## Backlinks {#backlinks}

-   [Silvanus Thompson | Calculus Made Easy]({{< relref "silvanus_thompson_calculus_made_easy.md" >}})
